- Added Min/Max example to ADTExamples.   There are still some artifacts from the previous ADT implementation,   I've commented those out at the end. - Added [refines_model_pickImpl] to ADT.Refinement which allows models   to be refined between Pick Implementations. - Added ADTExamples back to the makefile.

ADTExamples.v
@@ -5,9 +5,8 @@ Require Export ADT ADTRefinement.
 Generalizable All Variables.
 Set Implicit Arguments.
 
-(** * Basic ADT definitions *)
-Section comp_env.
-  (** * An example, composing binary commutative associative calculators for computable nat multisets *)
+Section BinOpSpec.
+  (** Specification for comparisions over a collection **)
 
   Definition multiset := nat -> nat.
   Definition add (s : multiset) (n : nat) : multiset
@@ -15,66 +14,299 @@ Section comp_env.
                 then S (s m)
                 else s m.
 
-  Require Import Min Max List.
-
-  Coercion sumbooltobool A B : {A} + {B} -> bool := fun x => if x then true else false.
-
-  Infix "<=" := le_dec : bool_scope.
-  Infix "<" := lt_dec : bool_scope.
-  Infix ">=" := ge_dec : bool_scope.
-  Infix ">" := gt_dec : bool_scope.
-
+  Global Arguments add s n / m.
+  
+  (* Specification for adding an element *)
   Definition add_spec : mutatorMethodSpec multiset
     := fun m x m' => forall k, m' k = (add m x) k.
 
-  Arguments add_spec / .
+  Arguments add_spec m x m' / .
 
-  Definition bin_op_spec (op : nat -> nat -> nat) (default_value : nat)
+  Variable opSpec : nat -> nat -> Prop.
+  Variable defaultSpec : nat -> Prop.
+
+  (* Specification for counting occurences of an element *)
+  Definition count_spec : observerMethodSpec multiset
+    := fun m x n => n = m x.
+  
+  Arguments count_spec / .
+
+  (* Specification for calculating op. *)
+
+  Definition bin_op_spec
   : observerMethodSpec multiset
-    := fun m x n => exists l : list nat,
-                      (forall v, m v = count_occ eq_nat_dec l v)
-                      /\ match l with
-                           | nil => n = default_value
-                           | cons z zs => n = fold_right op z zs
-                         end.
+    := fun m _ n => (defaultSpec n /\ forall n', m n' = 0) \/ (* Either the set is empty *)
+                    (m n > 0 /\ forall n', m n' > 0 -> opSpec n n'). (* Or n is the op-est thing in the set *)
 
   Arguments bin_op_spec / .
 
   Definition NatBinOpSpec
-             (op : nat -> nat -> nat)
-             (is_assoc : forall x y z, op x (op y z) = op (op x y) z)
-             (is_comm : forall x y, op x y = op y x)
-             (default_value : nat)
   : ADT
-    := pickImpl (fun _ : unit => add_spec) (fun _ : unit => bin_op_spec op default_value).
+    := pickImpl (fun _ : unit => add_spec) 
+                (fun _ : unit => bin_op_spec).
 
-  Local Obligation Tactic :=
-    eauto with arith;
-    try solve [ repeat match goal with
-                         | _ => progress (simpl; rewrite_hyp'; trivial)
-                         | [ |- _ -> _ ] => let x := fresh in intro x; induction x; trivial
-                       end
-              | intros; omega ].
+End BinOpSpec.
 
-  Program Definition NatLower default_value : ADT
-    := NatBinOpSpec min _ _ default_value.
+Definition NatLower : ADT 
+  := NatBinOpSpec le (fun n => True).  (* Spec for collection with lower bound. *)
 
-  Program Definition NatUpper default_value : ADT
-    := NatBinOpSpec max _ _ default_value.
+Definition NatUpper 
+: ADT := NatBinOpSpec ge (fun n => True).  (* Spec for collection with upper bound. *)
 
-  Program Definition NatSum default_value : ADT
-    := NatBinOpSpec plus _ _ default_value.
+Section BinOpImpl. 
+  (* Implementation of comparisions over a collection implemented as a list. *)
+  
+  Require Import List.
 
-  Program Definition NatProd default_value : ADT
-    := NatBinOpSpec mult _ _ default_value.
+  Variable op : nat -> nat -> nat.
+  Variable defaultValue : nat.
 
-  Hint Immediate le_min_l le_min_r le_max_l le_max_r.
+  Definition add_impl : mutatorMethodType (list nat)
+    := fun m x => ret (x :: m).
+
+  Arguments add_impl / .
+
+  Definition bin_op_impl : observerMethodType (list nat) 
+    := fun m _ => match m with 
+                    | [] => ret defaultValue  (* Only return default if collection is empty *)
+                    | a :: m' => ret (fold_left op m' a)
+                  end.
+                    
+  Arguments bin_op_impl / .
+
+  Definition NatBinOpImpl 
+  : ADT 
+    := {| Model := list nat;
+          MutatorIndex := unit;
+          ObserverIndex := unit;
+          MutatorMethods := fun _ => add_impl;
+          ObserverMethods := fun _ => bin_op_impl
+       |}.
+
+End BinOpImpl.  
+
+Section BinOpRefine.
+
+  Variable opSpec : nat -> nat -> Prop.
+  Variable defaultSpec : nat -> Prop.
+
+  Variable op : nat -> nat -> nat.
+  Variable defaultValue : nat. 
+
+  Hypothesis op_commutes : forall x y, op x y = op y x.
+  Hypothesis op_assoc : forall x y z, op (op x y) z = op x (op y z).
+  Hypothesis default_satisfies_defaultSpec : defaultSpec defaultValue.
+  Hypothesis op_returns_arg : forall n m,
+    op n m = n \/ op n m = m.
+  Hypothesis op_preserves_op1 : forall n m,
+    opSpec (op n m) m.
+  Hypothesis op_preserves_op2 : forall n m,
+    opSpec (op n m) n. 
+  Hypothesis op_refl : Reflexive opSpec.
+  Hypothesis op_trans : Transitive opSpec.
+
+  Lemma fold_left_op_preserves_opSpec l :
+    forall a n', opSpec a n' -> opSpec (fold_left op l a) n'.
+  Proof.
+    induction l; simpl; auto.
+    intros; eapply IHl; etransitivity; [ | eassumption]; eauto.
+  Qed.
+
+  Hint Resolve fold_left_op_preserves_opSpec.
+
+  Lemma fold_left_op_preserves_opSpec' l
+    : forall acc,
+      opSpec (fold_left op l acc) acc.
+  Proof.
+    eauto.
+  Qed.
+  
+  Hint Resolve fold_left_op_preserves_opSpec'.
+  
+  Lemma fold_left_op_In_preserves_opSpec : 
+    forall m n' a,
+      In n' m -> opSpec (fold_left op m a) n'.
+  Proof.
+    induction m; simpl; intuition; subst.
+    destruct (op_returns_arg a0 n'); rewrite H; eauto.
+    generalize (op_preserves_op1 a0 n'); rewrite H; eauto.
+  Qed.
+
+  Hint Resolve fold_left_op_In_preserves_opSpec.
+
+  Lemma fold_left_discards_less_oppy : 
+    forall m a, a <> fold_left op m a -> exists a', In (fold_left op m a) m /\ op a a' = a'.
+  Proof.
+    induction m; simpl; intuition.
+    destruct (op_returns_arg a0 a); rewrite H0 in *|-*; eauto.
+    destruct (IHm _ H) as [a' [In_a' op_a] ]; eauto.
+    destruct (eq_nat_dec a (fold_left op m a)); eauto.
+    destruct (IHm _ n); exists x; intuition.
+    rewrite <- H3, <- op_assoc, H0; auto.
+  Qed.
+
+  Lemma fold_left_constains_more_oppy : 
+    forall m a, a <> fold_left op m a -> count_occ eq_nat_dec m (fold_left op m a) > 0.
+  Proof.
+    intros m a neq; destruct (fold_left_discards_less_oppy m neq) as [a' [In_a' op_a] ].
+    eapply count_occ_In; eauto.
+  Qed.
+
+  Hint Resolve fold_left_constains_more_oppy.
+
+  Program Definition absList2Multiset (l : list nat) : multiset := count_occ eq_nat_dec l.
+
+  Arguments absList2Multiset l / n .
+  Arguments add_spec m x m' /.
+
+  Theorem refine_add_impl m n : 
+  refine {m' : list nat |
+          add_spec (absList2Multiset m) n (absList2Multiset m')}
+         (add_impl m n).
+  Proof.
+    intros v old_hyp.
+    apply computes_to_inv in old_hyp; simpl in old_hyp; subst.
+    constructor; simpl; auto.
+  Qed.
+
+  Hint Resolve refine_add_impl.
+
+  Arguments bin_op_spec opSpec defaultSpec m x n /.
+
+  Ltac find_if_inside :=
+    match goal with
+      | [ |- context[if ?X then _ else _] ] => destruct X
+      | [ H : context[if ?X then _ else _] |- _ ]=> destruct X
+    end.
+
+  Ltac substs :=
+    repeat (match goal with H: ?x = ?y |- _ => 
+            first [ subst x | subst y ] end).
+
+  Theorem refine_bin_op_impl m n : 
+  refine {m' : nat |
+          bin_op_spec opSpec defaultSpec (absList2Multiset m) n m'}
+         (bin_op_impl op defaultValue m n).
+  Proof.
+    intros v old_hyp.
+    apply computes_to_inv in old_hyp; simpl in old_hyp; subst.
+    constructor; simpl; auto.
+    destruct m; simpl in old_hyp; subst; intuition.
+    right; revert n0; induction m; simpl; [intuition; (find_if_inside; substs; intuition) | intuition].
+    - repeat (find_if_inside; substs; intuition).
+      destruct (op_returns_arg n0 a); rewrite H in *|-*; eauto.
+    - repeat find_if_inside; substs; eauto;
+      destruct (op_returns_arg n0 a); rewrite H0 in *|-*; eauto.
+      destruct (IHm n0) as [_ IHm']; specialize (IHm' n'); simpl in IHm';
+      find_if_inside; intuition.
+      destruct (IHm a) as [_ IHm']; specialize (IHm' n'); simpl in IHm';
+      find_if_inside; intuition.
+  Qed.      
+      
+  Lemma refines_NatBinOp 
+  : refineADT (NatBinOpSpec opSpec defaultSpec) (NatBinOpImpl op defaultValue).
+  Proof.
+    etransitivity.
+    eapply refines_model_pickImpl with 
+    (abs := absList2Multiset).
+    econstructor 1 with (abs := @Return (list nat))
+                          (mutatorMap := @id unit)
+                          (observerMap := @id unit); simpl; intros.
+    interleave_autorewrite_refine_monad_with ltac:(apply refine_add_impl).
+    interleave_autorewrite_refine_monad_with ltac:(apply refine_bin_op_impl).
+  Qed.
+
+End BinOpRefine.
+
+Section ImplExamples. 
+
+  Local Ltac induction_list_then tac :=
+    lazymatch goal with
+  | [ l : list _ |- _ ]
+    => repeat match goal with
+                | [ H : appcontext[l] |- _ ] => clear H
+              end;
+      induction l; tac
+  end.
+
+  Local Ltac manipulate_op op_assoc op_comm :=
+    match goal with
+      | _ => reflexivity
+      | _ => progress simpl in *
+      | _ => apply op_comm
+      | _ => rewrite <- ?op_assoc; revert op_assoc op_comm; rewrite_hyp'; intros
+      | _ => rewrite ?op_assoc; revert op_assoc op_comm; rewrite_hyp'; intros
+      | _ => rewrite <- ?op_assoc; f_equal; []
+      | _ => rewrite ?op_assoc; f_equal; []
+      | _ => apply op_comm
+    end.
+
+  Local Ltac deep_manipulate_op op op_assoc op_comm can_comm_tac :=
+    repeat match goal with
+             | _ => progress repeat manipulate_op op_assoc op_comm
+             | [ |- appcontext[op ?a ?b] ]
+               => can_comm_tac a b;
+                 rewrite (op_comm a b);
+                 let new_can_comm_tac :=
+                     fun x y =>
+                       can_comm_tac x y;
+                       try (unify x a;
+                            unify y b;
+                            fail 1 "Cannot commute" a "and" b "again")
+                 in deep_manipulate_op op op_assoc op_comm new_can_comm_tac
+           end.
+
+  Local Ltac solve_after_induction_list op op_assoc op_comm :=
+    solve [ deep_manipulate_op op op_assoc op_comm ltac:(fun a b => idtac) ].
+
+  Local Ltac t :=
+    repeat match goal with
+             | _ => assumption
+             | _ => intro
+             | _ => progress simpl in *
+             | [ |- appcontext[if string_dec ?A ?B then _ else _ ] ]
+               => destruct (string_dec A B)
+             | _ => progress subst
+             | [ H : ex _ |- _ ] => destruct H
+             | [ H : and _ _ |- _ ] => destruct H
+             | _ => split
+             | [ H : option _ |- _ ] => destruct H
+             | [ H : _ |- _ ] => solve [ inversion H ]
+             | [ |- appcontext[match ?x with _ => _ end] ] => destruct x
+             | [ H : appcontext[match ?x with _ => _ end] |- _  ] => destruct x
+             | [ H : Some _ = Some _ |- _ ] => inversion H; clear H
+             | _ => progress f_equal; []
+             | _ => progress intuition
+             | _ => repeat esplit; reflexivity
+             | [ H : _ |- _ ] => rewrite H; try (rewrite H; fail 1)
+           end.
+
+  Local Ltac t' op op_assoc op_comm :=
+    repeat first [ progress t
+                 | progress induction_list_then ltac:(solve_after_induction_list op op_assoc op_comm) ].
+
+  Require Import Min.        
 
   Lemma min_trans : forall n m v,
                       n <= v
                       -> min n m <= v.
     intros; destruct (min_spec n m); omega.
   Qed.
+  
+  Hint Resolve min_trans.
+
+  Definition MinCollection (defaultValue : nat) :
+    { Rep : ADT
+    | refineADT NatLower Rep }.
+  Proof.
+    eexists; eapply refines_NatBinOp with 
+             (op := min)
+               (defaultValue := defaultValue); t.    
+    rewrite min_assoc; auto.
+    edestruct min_dec; eauto.
+  Defined.
+
+  Require Import Max.
 
   Lemma max_trans : forall n m v,
                       n >= v
@@ -82,163 +314,220 @@ Section comp_env.
     intros; destruct (max_spec n m); omega.
   Qed.
 
-  Hint Resolve min_trans max_trans.
+  Hint Resolve max_trans.
 
-  Arguments add _ _ _ / .
+  Definition MaxCollection (defaultValue : nat) :
+    { Rep : ADT
+    | refineADT NatUpper Rep }.
+  Proof.
+    eexists; eapply refines_NatBinOp with 
+             (op := max)
+               (defaultValue := defaultValue); t.    
+    rewrite max_assoc; auto.
+    edestruct max_dec; eauto.
+  Defined.
 
-  Section def_NatBinOpI.
+End ImplExamples.
 
-    Local Ltac induction_list_then tac :=
-      lazymatch goal with
-  | [ l : list _ |- _ ]
-    => repeat match goal with
-                | [ H : appcontext[l] |- _ ] => clear H
-              end;
-      induction l; tac
-    end.
+(* Definition NatLower : ADT  *)
+(*   := NatBinOpSpec le (fun n => n = 0).  (* Spec for collection with lower bound. *) *)
 
-    Local Ltac manipulate_op op_assoc op_comm :=
-      match goal with
-        | _ => reflexivity
-        | _ => progress simpl in *
-        | _ => apply op_comm
-        | _ => rewrite <- ?op_assoc; revert op_assoc op_comm; rewrite_hyp'; intros
-        | _ => rewrite ?op_assoc; revert op_assoc op_comm; rewrite_hyp'; intros
-        | _ => rewrite <- ?op_assoc; f_equal; []
-        | _ => rewrite ?op_assoc; f_equal; []
-        | _ => apply op_comm
-      end.
-
-    Local Ltac deep_manipulate_op op op_assoc op_comm can_comm_tac :=
-      repeat match goal with
-               | _ => progress repeat manipulate_op op_assoc op_comm
-               | [ |- appcontext[op ?a ?b] ]
-                 => can_comm_tac a b;
-                   rewrite (op_comm a b);
-                   let new_can_comm_tac :=
-                       fun x y =>
-                         can_comm_tac x y;
-                         try (unify x a;
-                              unify y b;
-                              fail 1 "Cannot commute" a "and" b "again")
-                   in deep_manipulate_op op op_assoc op_comm new_can_comm_tac
-             end.
-
-    Local Ltac solve_after_induction_list op op_assoc op_comm :=
-      solve [ deep_manipulate_op op op_assoc op_comm ltac:(fun a b => idtac) ].
+(* Definition NatUpper  *)
+(* : ADT := NatBinOpSpec ge (fun n => n = 0).  (* Spec for collection with upper bound. *) *)
 
 
-    Local Ltac t :=
-      repeat match goal with
-               | _ => assumption
-               | _ => intro
-               | _ => progress simpl in *
-               | [ |- appcontext[if string_dec ?A ?B then _ else _ ] ]
-                 => destruct (string_dec A B)
-               | _ => progress subst
-               | [ H : ex _ |- _ ] => destruct H
-               | [ H : and _ _ |- _ ] => destruct H
-               | _ => split
-               | [ H : option _ |- _ ] => destruct H
-               | [ H : _ |- _ ] => solve [ inversion H ]
-               | [ |- appcontext[match ?x with _ => _ end] ] => destruct x
-               | [ H : appcontext[match ?x with _ => _ end] |- _  ] => destruct x
-               | [ H : Some _ = Some _ |- _ ] => inversion H; clear H
-               | _ => progress f_equal; []
-               | _ => progress intuition
-               | _ => repeat esplit; reflexivity
-               | [ H : _ |- _ ] => rewrite H; try (rewrite H; fail 1)
-             end.
+(* Definition NatLowerI defaultValue : ADT (NatLower defaultValue) *)
+(*   := NatBinOpI _ _ _ _. *)
 
-    Local Ltac t' op op_assoc op_comm :=
-      repeat first [ progress t
-                   | progress induction_list_then ltac:(solve_after_induction_list op op_assoc op_comm) ].
+(* Definition NatUpperI : ADTimpl (NatUpper default_val) *)
+(*   := NatBinOpI _ _ _ _. *)
 
-    Definition NatBinOpImpl op is_assoc is_comm default_value :  
-      { impl : ADT | refineADT impl (NatBinOpSpec op is_assoc is_comm default_value)}.
-    Proof.
-      eexists.
-      set_evars.
+(*   Program Definition NatUpper default_value : ADT *)
+(*     := NatBinOpSpec max default_value. *)
 
-      set_evars.
+(*   Program Definition NatSum default_value : ADT *)
+(*     := NatBinOpSpec plus default_value. *)
 
-    | forall l, refineADT { x : _ | is_min_max l x }%comp (f l) }.
-    Proof.
+(*   Program Definition NatProd default_value : ADT *)
+(*     := NatBinOpSpec mult default_value. *)
 
-    Definition NatBinOpImpl
-               (op : nat -> nat -> nat)
-               (is_assoc : forall x y z, op x (op y z) = op (op x y) z)
-               (is_comm : forall x y, op x y = op y x)
-               (default_value : nat) : ADT.
-    Proof.
-      intros.
-      refine {|
-          Model := option nat;
-          MutatorMethods u val x := (ret (match val with
-                                                 | None => Some x
-                                                 | Some x' => Some (op x x')
-                                               end,
-                                               0))%comp;
-          ObserverMethods u val x := (ret (val,
-                                                match val with
-                                                  | None => default_value
-                                                  | Some x => x
-                                                end))%comp
-        |};
-        intros [];
-        solve [ (intros m [n|] [l [H0 H1] ] x ? ?);
-                inversion_by computes_to_inv; subst; simpl in *;
-                (exists (add m x));
-                repeat split;
-                try (exists (x::l));
-                abstract t' op op_assoc op_comm
-              | intros m [n|] [l [H0 H1] ] x ? ?;
-                       inversion_by computes_to_inv; subst; simpl in *;
-                repeat (split || exists m || exists l);
-                abstract t' op op_assoc op_comm
-              | intros m [n|] [l [H0 H1] ] x ? ?;
-                       inversion_by computes_to_inv; subst; simpl in *;
-                [ repeat split;
-                  try (exists (add (fun _ => 0) n));
-                  repeat split;
-                  try (exists (n::nil));
-                  abstract (repeat split)
-                | repeat split;
-                  try (exists m);
-                  repeat split;
-                  try (exists l);
-                  abstract (repeat split; assumption) ]
-              ].
-    Defined.
-  End def_NatBinOpI.
+(*   Hint Immediate le_min_l le_min_r le_max_l le_max_r. *)
 
-  Section nat_op_ex.
-    Variable default_val : nat.
+(*   Lemma min_trans : forall n m v, *)
+(*                       n <= v *)
+(*                       -> min n m <= v. *)
+(*     intros; destruct (min_spec n m); omega. *)
+(*   Qed. *)
 
-    Definition NatLowerI : ADTimpl (NatLower default_val)
-      := NatBinOpI _ _ _ _.
+(*   Lemma max_trans : forall n m v, *)
+(*                       n >= v *)
+(*                       -> max n m >= v. *)
+(*     intros; destruct (max_spec n m); omega. *)
+(*   Qed. *)
 
-    Definition NatUpperI : ADTimpl (NatUpper default_val)
-      := NatBinOpI _ _ _ _.
+(*   Hint Resolve min_trans max_trans. *)
 
-    Definition NatSumI : ADTimpl (NatSum default_val)
-      := NatBinOpI _ _ _ _.
+(*   Arguments add _ _ _ / . *)
 
-    Definition NatProdI : ADTimpl (NatProd default_val)
-      := NatBinOpI _ _ _ _.
-  End nat_op_ex.
 
-  Local Open Scope string_scope.
+(*   Section def_NatBinOpI. *)
 
-  Definition NatSumProd_spec : ADT
-    := {| Model := multiset;
-          MutatorIndex := unit;
-          ObserverIndex := unit + unit;
-          MutatorMethodSpecs u := add_spec;
-          ObserverMethodSpecs u m x n :=
-            match u with
-              | inl _ => bin_op_spec plus 0 m x n
-              | inr _ => bin_op_spec mult 1 m x n
-            end
-       |}.
-End comp_env.
+(*     Local Ltac induction_list_then tac := *)
+(*       lazymatch goal with *)
+(*   | [ l : list _ |- _ ] *)
+(*     => repeat match goal with *)
+(*                 | [ H : appcontext[l] |- _ ] => clear H *)
+(*               end; *)
+(*       induction l; tac *)
+(*     end. *)
+
+(*     Local Ltac manipulate_op op_assoc op_comm := *)
+(*       match goal with *)
+(*         | _ => reflexivity *)
+(*         | _ => progress simpl in * *)
+(*         | _ => apply op_comm *)
+(*         | _ => rewrite <- ?op_assoc; revert op_assoc op_comm; rewrite_hyp'; intros *)
+(*         | _ => rewrite ?op_assoc; revert op_assoc op_comm; rewrite_hyp'; intros *)
+(*         | _ => rewrite <- ?op_assoc; f_equal; [] *)
+(*         | _ => rewrite ?op_assoc; f_equal; [] *)
+(*         | _ => apply op_comm *)
+(*       end. *)
+
+(*     Local Ltac deep_manipulate_op op op_assoc op_comm can_comm_tac := *)
+(*       repeat match goal with *)
+(*                | _ => progress repeat manipulate_op op_assoc op_comm *)
+(*                | [ |- appcontext[op ?a ?b] ] *)
+(*                  => can_comm_tac a b; *)
+(*                    rewrite (op_comm a b); *)
+(*                    let new_can_comm_tac := *)
+(*                        fun x y => *)
+(*                          can_comm_tac x y; *)
+(*                          try (unify x a; *)
+(*                               unify y b; *)
+(*                               fail 1 "Cannot commute" a "and" b "again") *)
+(*                    in deep_manipulate_op op op_assoc op_comm new_can_comm_tac *)
+(*              end. *)
+
+(*     Local Ltac solve_after_induction_list op op_assoc op_comm := *)
+(*       solve [ deep_manipulate_op op op_assoc op_comm ltac:(fun a b => idtac) ]. *)
+
+(*     Local Ltac t := *)
+(*       repeat match goal with *)
+(*                | _ => assumption *)
+(*                | _ => intro *)
+(*                | _ => progress simpl in * *)
+(*                | [ |- appcontext[if string_dec ?A ?B then _ else _ ] ] *)
+(*                  => destruct (string_dec A B) *)
+(*                | _ => progress subst *)
+(*                | [ H : ex _ |- _ ] => destruct H *)
+(*                | [ H : and _ _ |- _ ] => destruct H *)
+(*                | _ => split *)
+(*                | [ H : option _ |- _ ] => destruct H *)
+(*                | [ H : _ |- _ ] => solve [ inversion H ] *)
+(*                | [ |- appcontext[match ?x with _ => _ end] ] => destruct x *)
+(*                | [ H : appcontext[match ?x with _ => _ end] |- _  ] => destruct x *)
+(*                | [ H : Some _ = Some _ |- _ ] => inversion H; clear H *)
+(*                | _ => progress f_equal; [] *)
+(*                | _ => progress intuition *)
+(*                | _ => repeat esplit; reflexivity *)
+(*                | [ H : _ |- _ ] => rewrite H; try (rewrite H; fail 1) *)
+(*              end. *)
+
+(*     Local Ltac t' op op_assoc op_comm := *)
+(*       repeat first [ progress t *)
+(*                    | progress induction_list_then ltac:(solve_after_induction_list op op_assoc op_comm) ]. *)
+
+(*     Definition NatBinOpImpl *)
+(*                (op : nat -> nat -> nat) *)
+(*                (default_value : nat) : ADT. *)
+(*     Proof. *)
+(*       intros. *)
+(*       refine {|  *)
+(*           Model := option nat; *)
+(*           MutatorIndex := unit; *)
+(*           ObserverIndex := unit; *)
+(*           MutatorMethods u val x := ret (match val with  *)
+(*                                              | None => Some x *)
+(*                                              | Some x' => Some (op x x') *)
+(*                                          end)%comp; *)
+(*           ObserverMethods u val x := ret (match val with  *)
+(*                                               | None => default_value *)
+(*                                               | Some x => x *)
+(*                                           end) *)
+(*         |}. *)
+(*     Defined. *)
+
+(*   End def_NatBinOpI. *)
+
+(*       Print ADT. *)
+(*       intros []. *)
+                                        
+(*       refine {| *)
+(*           Model := option (nat * nat); *)
+(*           MutatorMethods u val x := (ret (match val with *)
+(*                                                  | None => Some x *)
+(*                                                  | Some x' => Some (op x (fst x')) *)
+(*                                                end, *)
+(*                                                0))%comp; *)
+(*           ObserverMethods u val x := (ret (val, *)
+(*                                                 match val with *)
+(*                                                   | None => default_value *)
+(*                                                   | Some x => x *)
+(*                                                 end))%comp *)
+(*         |}; *)
+(*         intros []; *)
+(*         solve [ (intros m [n|] [l [H0 H1] ] x ? ?); *)
+(*                 inversion_by computes_to_inv; subst; simpl in *; *)
+(*                 (exists (add m x)); *)
+(*                 repeat split; *)
+(*                 try (exists (x::l)); *)
+(*                 abstract t' op op_assoc op_comm *)
+(*               | intros m [n|] [l [H0 H1] ] x ? ?; *)
+(*                        inversion_by computes_to_inv; subst; simpl in *; *)
+(*                 repeat (split || exists m || exists l); *)
+(*                 abstract t' op op_assoc op_comm *)
+(*               | intros m [n|] [l [H0 H1] ] x ? ?; *)
+(*                        inversion_by computes_to_inv; subst; simpl in *; *)
+(*                 [ repeat split; *)
+(*                   try (exists (add (fun _ => 0) n)); *)
+(*                   repeat split; *)
+(*                   try (exists (n::nil)); *)
+(*                   abstract (repeat split) *)
+(*                 | repeat split; *)
+(*                   try (exists m); *)
+(*                   repeat split; *)
+(*                   try (exists l); *)
+(*                   abstract (repeat split; assumption) ] *)
+(*               ]. *)
+(*     Defined. *)
+(*   End def_NatBinOpI. *)
+
+(*   Section nat_op_ex. *)
+(*     Variable default_val : nat. *)
+
+(*     Definition NatLowerI : ADTimpl (NatLower default_val) *)
+(*       := NatBinOpI _ _ _ _. *)
+
+(*     Definition NatUpperI : ADTimpl (NatUpper default_val) *)
+(*       := NatBinOpI _ _ _ _. *)
+
+(*     Definition NatSumI : ADTimpl (NatSum default_val) *)
+(*       := NatBinOpI _ _ _ _. *)
+
+(*     Definition NatProdI : ADTimpl (NatProd default_val) *)
+(*       := NatBinOpI _ _ _ _. *)
+(*   End nat_op_ex. *)
+
+(*   Local Open Scope string_scope. *)
+
+(*   Definition NatSumProd_spec : ADT *)
+(*     := {| Model := multiset; *)
+(*           MutatorIndex := unit; *)
+(*           ObserverIndex := unit + unit; *)
+(*           MutatorMethodSpecs u := add_spec; *)
+(*           ObserverMethodSpecs u m x n := *)
+(*             match u with *)
+(*               | inl _ => bin_op_spec plus 0 m x n *)
+(*               | inr _ => bin_op_spec mult 1 m x n *)
+(*             end *)
+(*        |}. *)
